---
title: "formula for posterior distribution"
author: "Paulina Han"
date: '2022-05-04'
output: html_document
---

## Posterior dist of $\mu$
$$
\begin{aligned}
 f(\mu | B ,\Sigma, \sigma^2, Y)  & \propto exp(-\frac{1}{2} \sum_{i=1}^N ( \beta_{i} - \mu)^{T} \Sigma^{-1}(\beta{i} - \mu)) \\
 & \propto exp( \frac{1}{2} ( \sum_{i=1}^N \beta_{i}^{T}\Sigma^{-1}\beta_{i} + \mu^{T}N\Sigma^{-1}\mu - 2\sum_{i=1}^N\beta_{i}^{T}\Sigma^{-1}\mu)) \\
 & \propto exp(R + \beta V \beta -2M \beta) \\
 & \propto exp((\beta - V^{-1}M)^{T} V (\beta - V^{-1}M)) \\
& \implies \mu \sim MVN(V^{-1}M, V^{-1}) \\
\text{where:  }
V &= N\Sigma^{-1} \\
R &= \sum_{i=1}^N \beta_{i}^{T}\Sigma^{-1}\beta_{i} \\
M &= \sum_{i=1}^N \Sigma^{-1}\beta_{i} \\

\end{aligned}
$$
